some experiments

tools/Vale/test/Semantics.fst
@@ -61,7 +61,6 @@ type ocmp =
   | OLt: o1:operand -> o2:operand -> ocmp
   | OGt: o1:operand -> o2:operand -> ocmp
 
-
 type ins =
   | Mov64      : dst:dst_op -> src:operand -> ins
   | Add64      : dst:dst_op -> src:operand -> ins
@@ -99,56 +98,130 @@ noeq type state = {
 
 assume val havoc : state -> ins -> Tot nat64
 
-(*
- * writing all the functions as Tot functions
- *)
-let eval_reg (r:reg) (s:state) :nat64 =
-  s.regs.[r]
+type reader (a:Type) = state -> a
 
-(*
-let valid_resolved_addr (ptr:int) (m:mem) :bool =
-  m `contains` ptr /\
-  m `contains` ptr + 1 /\
-  m `contains` ptr + 2 /\
-  m `contains` ptr + 3 
-*)
+noeq type eval_t = {
+  get_flags   :unit -> reader nat64;
+  eval_reg    :reg -> reader nat64;
+  eval_mem    :int -> reader nat64;
+  eval_maddr  :maddr -> reader int;
+  eval_operand:operand -> reader nat64;
+  eval_ocmp   :ocmp -> reader bool
+}
 
-let eval_mem (ptr:int) (s:state) :nat64 =
-  s.mem.[ptr]
+let eval :eval_t =
+  let return (#a:Type) (x:a) :reader a = fun s -> x in
+  let bind (#a:Type) (#b:Type) (f:reader a) (g:a -> reader b) :reader b =
+    fun s -> let x = f s in
+          g x s
+  in
+  let get () :reader state = fun s -> s in
 
-let eval_maddr (m:maddr) (s:state) :int =
-  let open FStar.Mul in
+  let get_flags :unit -> reader nat64 = fun _ -> s <-- get (); return s.flags in
+  let eval_reg :reg -> reader nat64 = fun r -> s <-- get (); return s.regs.[r] in
+  let eval_mem :int -> reader nat64 = fun ptr -> s <-- get (); return s.mem.[ptr] in
+  let eval_maddr :maddr -> reader int = fun m ->
+    let open FStar.Mul in
     match m with
-    | MConst n -> n
-    | MReg reg offset -> (eval_reg reg s) + offset
-    | MIndex base scale index offset -> eval_reg base s + scale * eval_reg index s + offset
+    | MConst n -> return n
+    | MReg r offset ->
+      x <-- eval_reg r;
+      return (x + offset)
+    | MIndex base scale index offset ->
+      x <-- eval_reg base;
+      y <-- eval_reg index;    
+      return (x + scale * y + offset)
+  in
+  let eval_operand :operand -> reader nat64 = fun o ->
+    match o with
+    | OConst n -> return n
+    | OReg r   -> eval_reg r
+    | OMem m   ->
+      x <-- eval_maddr m;
+      eval_mem x
+  in
+  let eval_ocmp :ocmp -> reader bool = fun c ->
+    match c with
+    | OEq o1 o2 -> 
+      x <-- eval_operand o1;
+      y <-- eval_operand o2;
+      return (x = y)
+    | ONe o1 o2 -> 
+      x <-- eval_operand o1;
+      y <-- eval_operand o2;
+      return (x <> y)
+    | OLe o1 o2 ->
+      x <-- eval_operand o1;
+      y <-- eval_operand o2;
+      return (x <= y)
+    | OGe o1 o2 ->
+      x <-- eval_operand o1;
+      y <-- eval_operand o2;
+      return (x >= y)
+    | OLt o1 o2 ->
+      x <-- eval_operand o1;
+      y <-- eval_operand o2;
+      return (x < y)
+    | OGt o1 o2 ->
+      x <-- eval_operand o1;
+      y <-- eval_operand o2;
+      return (x > y)
+  in
 
-let eval_operand (o:operand) (s:state) :nat64 =
+  {
+    get_flags = get_flags;
+    eval_reg = eval_reg;
+    eval_mem = eval_mem;
+    eval_maddr = eval_maddr;
+    eval_operand = eval_operand;
+    eval_ocmp = eval_ocmp
+  }
+
+type st (a:Type) = state -> (option a * state)
+
+unfold let lift (#a:Type) (f:reader a) :st a =
+  fun s -> let x = f s in
+        (Some x, s)
+
+unfold let return (#a:Type) (x:a) :st a =
+  fun s -> (Some x, s)
+
+unfold let bind (#a:Type) (#b:Type) (f:st a) (g:a -> st b) :st b =
+  fun s ->
+    let (x_opt, s) = f s in
+    if None? x_opt then (None, { s with ok = false})
+    else g (Some?.v x_opt) s
+
+let get () :st state =
+  fun s -> (Some s, s)
+  
+let set (s:state) :st unit =
+  fun _ -> (Some (), s)
+  
+let fail () :st unit =
+  s <-- get ();
+  set ({s with ok = false})
+
+let update_reg (r:reg) (v:nat64) :st unit =
+  s <-- get ();
+  set ({s with regs = s.regs.[r] <- v})
+
+let update_mem (ptr:int) (v:nat64) :st unit =
+  s <-- get ();
+  set ({s with mem = s.mem.[ptr] <- v})
+
+let update_operand_preserve_flags' (o:dst_op) (v:nat64) :st unit =
   match o with
-  | OConst n -> n
-  | OReg r   -> eval_reg r s
-  | OMem m   -> eval_mem (eval_maddr m s) s
+  | OReg r   -> update_reg r v
+  | OMem m   ->
+    x <-- lift (eval.eval_maddr m);
+    update_mem x v
 
-let eval_ocmp (s:state) (c:ocmp) :bool =
-  match c with
-  | OEq o1 o2 -> eval_operand o1 s = eval_operand o2 s
-  | ONe o1 o2 -> eval_operand o1 s <> eval_operand o2 s
-  | OLe o1 o2 -> eval_operand o1 s <= eval_operand o2 s
-  | OGe o1 o2 -> eval_operand o1 s >= eval_operand o2 s
-  | OLt o1 o2 -> eval_operand o1 s < eval_operand o2 s
-  | OGt o1 o2 -> eval_operand o1 s > eval_operand o2 s
-
-let update_reg' (r:reg) (v:nat64) (s:state) :state = { s with regs = s.regs.[r] <- v }
-
-let update_mem (ptr:int) (v:nat64) (s:state) :state = { s with mem = s.mem.[ptr] <- v }
-
-let update_operand_preserve_flags' (o:dst_op) (v:nat64) (s:state) :state =
-  match o with
-  | OReg r   -> update_reg' r v s
-  | OMem m   -> update_mem (eval_maddr m s) v s
-
-let update_operand' (o:dst_op) (ins:ins) (v:nat64) (s:state) :state =
-  { (update_operand_preserve_flags' o v s) with flags = havoc s ins }
+let update_operand' (o:dst_op) (ins:ins) (v:nat64) :st unit =
+  s0 <-- get ();
+  update_operand_preserve_flags' o v;;
+  s1 <-- get ();
+  set ({s1 with flags = havoc s0 ins})
 
 (* REVIEW: Will we regret exposing a mod here?  Should flags be something with more structure? *)
 let cf (flags:nat64) :bool =
@@ -166,44 +239,32 @@ let update_cf (flags:nat64) (new_cf:bool) : (new_flags:nat64{cf new_flags == new
     else
       flags
 
-let valid_maddr (m:maddr) (s:state) :bool =
-  s.mem `contains` (eval_maddr m s)
+let check (b:bool) :st unit =
+  if b then return () else fail ()
 
-let valid_operand (o:operand) (s:state) :bool =
-  not (OMem? o) || (OMem? o && valid_maddr (OMem?.m o) s)
+let valid_maddr_b (m:maddr) (s:state) :bool =
+  let x = eval.eval_maddr m s in
+  s.mem `contains` x
 
-let valid_shift_operand (o:operand) (s:state) :bool =
+let valid_maddr (m:maddr) :st unit =
+  s <-- get ();
+  check (valid_maddr_b m s)
+
+let valid_operand_b (o:operand) (s:state) :bool =
+  not (OMem? o) || (OMem? o && valid_maddr_b (OMem?.m o) s)
+
+let valid_operand (o:operand) :st unit =
+  s <-- get ();
+  check (valid_operand_b o s)
+
+let valid_shift_operand_b (o:operand) (s:state) :bool =
   (OConst? o && 0 <= OConst?.n o && OConst?.n o < 32) 
   || 
-  ((OReg? o) && (Rcx? (OReg?.r o)) && eval_operand o s < nat32_max)
+  ((OReg? o) && (Rcx? (OReg?.r o)) && eval.eval_operand o s < nat32_max)
 
-
-let st (a:Type) = state -> option (a * state)
-
-unfold let return (#a:Type) (x:a) :st a =
-  fun s -> Some (x, s)
-
-unfold let bind (#a:Type) (#b:Type) (m:st a) (f:a -> st b) :st b =
-  fun s ->
-    match m s with
-    | None        -> None
-    | Some (x, s) -> f x s
-
-let get () :st state =
-  fun s -> Some (s, s)
-  
-let set (s:state) :st unit =
-  fun _ -> Some ((), s)
-  
-let fail () :st unit =
-  fun s -> None
-  
-let check (valid: state -> bool) :st unit =
-  s <-- get();
-  if valid s then
-    return ()
-  else 
-    fail ()
+let valid_shift_operand (o:operand) :st unit =
+  s <-- get ();
+  check (valid_shift_operand_b o s)
 
 (*
 let check_eval_operand (valid: operand -> state -> bool) (o:operand) : nat64 * st =
@@ -215,34 +276,25 @@ let check_eval_operand (valid: operand -> state -> bool) (o:operand) : nat64 * s
 *)
 
 let update_operand_preserve_flags (dst:dst_op) (v:nat64) :st unit =
- check (valid_operand dst);;  
-  s <-- get ();
-  set (update_operand_preserve_flags' dst v s)
+  valid_operand dst;;
+  update_operand_preserve_flags' dst v
 
 (* Default version havocs flags *)
 let update_operand (dst:dst_op) (ins:ins) (v:nat64) :st unit =
- check (valid_operand dst);;
-  s <-- get ();
-  set (update_operand' dst ins v s)
-
-let update_reg (r:reg) (v:nat64) :st unit =
-  s <-- get();
-  set (update_reg' r v s)
+  valid_operand dst;;
+  update_operand' dst ins v
 
 let update_flags (new_flags:nat64) :st unit =
   s <-- get();
   set ( { s with flags = new_flags } )
 
 let example (dst:dst_op) (src:operand) :st unit =
-  check (valid_operand dst);;
-  check (valid_operand src);;
+  valid_operand dst;;
+  valid_operand src;;
   update_operand_preserve_flags dst 2
 
 let test (dst:dst_op) (src:operand) (s:state) :state =
-  let maybe_s = (example dst src) s in
-    match maybe_s with
-    | None             -> { s with ok = false }
-    | Some ((), s_new) -> s_new
+   snd ((example dst src) s)
 
 open FStar.Mul
 
@@ -250,63 +302,82 @@ open FStar.Mul
 let eval_ins (ins:ins) (s:state) :state =
   if not s.ok then s
   else
-    let maybe_s = 
-      (match ins with 
-       | Mov64 dst src -> 
-	 check (valid_operand src);;
-	 update_operand_preserve_flags dst (eval_operand src s)
+  snd ((match ins with 
+  | Mov64 dst src ->
+    valid_operand src;;
+    x <-- lift (eval.eval_operand src);
+    update_operand_preserve_flags dst x
 
-       | Add64 dst src -> 
-	 check (valid_operand src);;
-	 update_operand dst ins ((eval_operand dst s + eval_operand src s) % nat64_max)
-			 
-       | AddLea64 dst src1 src2 -> 
-	 check (valid_operand src1);;
-	 check (valid_operand src2);;
-	 update_operand_preserve_flags dst ((eval_operand src1 s + eval_operand src2 s) % nat64_max)
-	 
-       | AddCarry64 dst src -> 
-	 let old_carry = if cf(s.flags) then 1 else 0 in
-	 let sum = eval_operand dst s + eval_operand src s + old_carry in
-	 let new_carry = sum >= nat64_max in
-	 check (valid_operand src);;
-	 update_operand dst ins (sum % nat64_max);;
-	 update_flags (update_cf s.flags new_carry)
+  | Add64 dst src -> 
+    valid_operand src;;
+    x <-- lift (eval.eval_operand dst);
+    y <-- lift (eval.eval_operand src);
+    update_operand dst ins ((x + y) % nat64_max)
+  
+  | AddLea64 dst src1 src2 ->
+    valid_operand src1;;
+    valid_operand src2;;
+    x <-- lift (eval.eval_operand src1);
+    y <-- lift (eval.eval_operand src2);
+    update_operand_preserve_flags dst ((x + y) % nat64_max)
 
-       | Sub64 dst src -> 
-	 check (valid_operand src);;
-	 update_operand dst ins ((eval_operand dst s - eval_operand src s) % nat64_max)
-	 
-       | Mul64 src -> 
-	 let product = eval_reg Rax s * eval_operand src s in
-	 let hi = product / nat64_max in
-	 let lo = product % nat64_max in
-	 check (valid_operand src);;
-	 update_reg Rax lo;;
-	 update_reg Rdx hi;;
-	 update_flags (havoc s ins)
-	   
-       | IMul64 dst src -> 
-	 check (valid_operand src);;
-	 update_operand dst ins ((eval_operand dst s * eval_operand src s) % nat64_max)	  
-	 
-       | Xor64 dst src -> 
-	 check (valid_operand src);;
-	 update_operand dst ins (FStar.UInt.logxor #64 (eval_operand dst s) (eval_operand src s))	  
-	 
-       | Shr64 dst amt -> 
-	 check (valid_shift_operand amt);;
-	 update_operand dst ins (FStar.UInt.shift_right #64 (eval_operand dst s) (eval_operand amt s))
+  | AddCarry64 dst src ->
+    flags <-- lift (eval.get_flags ());
+    x <-- lift (eval.eval_operand dst);
+    y <-- lift (eval.eval_operand src);
+    
+    let old_carry = if cf flags then 1 else 0 in
+    let sum = x + y + old_carry in
+    let new_carry = sum >= nat64_max in
+    
+    valid_operand src;;
+    update_operand dst ins (sum % nat64_max);;
+    update_flags (update_cf flags new_carry)
+    
+  | Sub64 dst src ->
+    valid_operand src;;
+    x <-- lift (eval.eval_operand dst);
+    y <-- lift (eval.eval_operand src);
+    update_operand dst ins ((x - y) % nat64_max)
 
-       | Shl64 dst amt ->
-	 check (valid_shift_operand amt);;
-	 update_operand dst ins (FStar.UInt.shift_left #64 (eval_operand dst s) (eval_operand amt s))
+  | Mul64 src ->
+    s <-- get ();
+    x <-- lift (eval.eval_reg Rax);
+    y <-- lift (eval.eval_operand src);
+    
+    let product = x * y in
+    let hi = product / nat64_max in
+    let lo = product % nat64_max in
+    
+    valid_operand src;;
+    update_reg Rax lo;;
+    update_reg Rdx hi;;
+    update_flags (havoc s ins)
 
-      ) s
-    in
-      match maybe_s with
-      | None             -> { s with ok = false }
-      | Some ((), s_new) -> s_new
+  | IMul64 dst src ->
+    valid_operand src;;
+    x <-- lift (eval.eval_operand dst);
+    y <-- lift (eval.eval_operand src);
+    update_operand dst ins ((x * y) % nat64_max)
+
+  | Xor64 dst src ->
+    valid_operand src;;
+    x <-- lift (eval.eval_operand dst);
+    y <-- lift (eval.eval_operand src);
+    update_operand dst ins (FStar.UInt.logxor #64 x y)
+	 
+  | Shr64 dst amt ->
+    valid_shift_operand amt;;
+    x <-- lift (eval.eval_operand dst);
+    y <-- lift (eval.eval_operand amt);
+    update_operand dst ins (FStar.UInt.shift_right #64 x y)
+
+  | Shl64 dst amt ->
+    valid_shift_operand amt;;
+    x <-- lift (eval.eval_operand dst);
+    y <-- lift (eval.eval_operand amt);
+    update_operand dst ins (FStar.UInt.shift_left #64 x y)) s)
+
 (*
     match ins with 
     | Mov64 dst src -> if valid_operand dst s && valid_operand src s then      
@@ -342,7 +413,7 @@ let eval_ins (ins:ins) (s:state) :state =
 let decr (c:code) (s:state) :nat =
   match c with
   | While _ _ inv ->
-    let n = eval_operand inv s in
+    let n = eval.eval_operand inv s in
     if n >= 0 then n else 0
   | _             -> 0
 
@@ -359,7 +430,9 @@ let rec eval_code c s =
   match c with
   | Ins ins                       -> Some (eval_ins ins s)
   | Block l                       -> eval_codes l s
-  | IfElse ifCond ifTrue ifFalse  -> if eval_ocmp s ifCond then eval_code ifTrue s else eval_code ifFalse s
+  | IfElse ifCond ifTrue ifFalse  ->
+    let b = eval.eval_ocmp ifCond s in
+    if b then eval_code ifTrue s else eval_code ifFalse s
   | While _ _ _                   -> eval_while c s
     
 and eval_codes l s =
@@ -371,8 +444,8 @@ and eval_codes l s =
     
 and eval_while c s_0 = (* trying to mimic the eval_while predicate using a function *)
   let While cond body inv = c in
-  let n_0 = eval_operand inv s_0 in
-  let b = eval_ocmp s_0 cond in
+  let n_0 = eval.eval_operand inv s_0 in
+  let b = eval.eval_ocmp cond s_0 in
 
   if n_0 <= 0 then
     if b then None else Some s_0  //if loop invariant is <= 0, the guard must be false
@@ -385,6 +458,27 @@ and eval_while c s_0 = (* trying to mimic the eval_while predicate using a funct
         let s_1 = Some?.v s_opt in
 	if not s_1.ok then Some s_1  //this is from the reference semantics, if ok flag is unset, return
 	else
-	  let n_1 = eval_operand inv s_1 in
+	  let n_1 = eval.eval_operand inv s_1 in
 	  if n_1 >= n_0 then None  //loop invariant must decrease
 	  else eval_while c s_1
+
+  (* let While cond body inv = c in *)
+  (* let n_0 = eval.eval_operand inv s_0 in *)
+  (* let (b_opt, s_0) = eval_ocmp cond s_0 in *)
+  (* match b_opt with *)
+  (* | None   -> Some ({ s_0 with ok = false }) *)
+  (* | Some b -> *)
+  (*   if n_0 <= 0 then *)
+  (*     if b then None else Some s_0  //if loop invariant is <= 0, the guard must be false *)
+  (*   else  //loop invariant > 0 *)
+  (*     if not b then None  //guard must evaluate to true *)
+  (*     else *)
+  (*       let s_opt = eval_code body s_0 in *)
+  (*       if None? s_opt then None *)
+  (*       else *)
+  (*         let s_1 = Some?.v s_opt in *)
+  (* 	  if not s_1.ok then Some s_1  //this is from the reference semantics, if ok flag is unset, return *)
+  (* 	  else *)
+  (* 	    let n_1 = eval_operand inv s_1 in *)
+  (* 	    if n_1 >= n_0 then None  //loop invariant must decrease *)
+  (* 	    else eval_while c s_1 *)
